strandspaceNSL.v
@@ -1,4 +1,3 @@
-
 Require Import Logic List ListSet Arith Peano_dec Omega Ensembles.
 Require Import Finite_sets_facts Finite_sets Relation_Definitions.
 Require Import Relation_Operators.
@@ -6,92 +5,49 @@ Require Import strictorder set_rep_equiv util.
 Require Import finite_set_builder strandlib.
 Require Import LibTactics.
 
-
 Require Import strandspace.
 
-Section NSLSpace.
+Module NSLSpace.
 
 Open Scope list_scope.
 Import ListNotations.
 Open Scope ss_scope.
 
-Hypothesis PModel : PenetratorModel = DolevYao.
+(* Names and Nonces *)
 Variable A B Na Nb : Text.
   Hypothesis neqANa : A <> Na.
   Hypothesis neqANb : A <> Nb.
   Hypothesis neqBNa : B <> Na.
   Hypothesis neqBNb : B <> Nb.
-Variable Ka Kb : Key.
+(* "Public" and "Private" keys *)
+Variable Ka Kb Ka' Kb' : Key.
   Hypothesis keyinj : Ka = Kb -> A = B.
+  Hypothesis Ka_inv : Inv Ka Ka'.
+  Hypothesis Kb_inv : Inv Kb Kb'.
+
+(* Self-communication in this protocol is nonsensical *)
+Hypothesis neqAB : A <> B. 
+
+Lemma neqKaKb : Ka <> Kb.
+Proof.
+  intros contra. 
+  apply keyinj in contra.
+  apply neqAB. auto.
+Qed.
+
+Definition NSLInitiator : Strand :=  
+  [(+ {(!Na) * (!A)}^[Kb]) ; 
+   (- {(!Na) * (!Nb) * (!B)}^[Ka]) ;
+   (+ {(!Nb)}^[Kb])].
+
+Definition NSLResponder : Strand :=  
+  [(- {(!Na) * (!A)}^[Kb]) ; 
+   (+ {(!Na) * (!Nb) * (!B)}^[Ka]) ;
+   (- {(!Nb)}^[Kb])].
 
 Hypothesis NSLProtocol : 
-  Protocol = [[(+ {(!Na) * (!A)}^[Kb]) ; 
-               (- {(!Na) * (!Nb) * (!B)}^[Ka]) ;
-               (+ {(!Nb)}^[Kb])] ; 
-              [(- {(!Na) * (!A)}^[Kb]) ; 
-               (+ {(!Na) * (!Nb) * (!B)}^[Ka]) ;
-               (- {(!Nb)}^[Kb])]].
-
-Definition s : Strand :=  [(- {(!Na) * (!A)}^[Kb]) ; 
-               (+ {(!Na) * (!Nb) * (!B)}^[Ka]) ;
-               (- {(!Nb)}^[Kb])].
-
-
-(* Proposition 5.2
-   Suppose:
-   1) The SS is an NSL space, C is a bundle in it,
-      and s is a responder strand
-      Resp[A, B, Na, Nb] with C-height 3. 
-   2) inv(Ka) is not in Kp
-   3) Na <> Nb and Nb is uniquely originating in the space. 
-   THEN
-    C contains an initiator's strand t (Init[A, B, Na, Nb] with 
-    C-height 3. *)
-
-Lemma s_regular : RegularStrand s.
-Proof.
-  unfold RegularStrand. rewrite NSLProtocol.
-  unfold s. right. left. reflexivity.
-Qed.
-
-Lemma s_height : length s = 3.
-Proof.
-  simpl. auto.
-Qed.
-
-Variable n0 : Node.
-Hypothesis n0_def : strand n0 = s /\
-                    index n0 = 1.
-Variable v0 : Msg.
-Hypothesis v0_def : msg n0 = v0.
-
-Lemma v0_val : v0 = {(!Na) * (!Nb) * (!B)}^[Ka].
-Proof.
-  destruct n0_def.
-  forwards*: (nth_node n0 s 1).
-  forwards: (node_smsg_msg_tx n0). eauto.
-  congruence.
-Qed.
-
-Variable n3 : Node.
-Hypothesis n3_def : strand n3 = s /\
-                    index n3 = 2.
-Variable v3 : Msg.
-Hypothesis v3_def : msg n3 = v3.
-
-Lemma v3_val : v3 = {(!Nb)}^[Kb].
-Proof.
-  destruct n3_def.
-  forwards*: (nth_node n3 s 2).
-  forwards: (node_smsg_msg_rx n3). eauto.
-  congruence.
-Qed.  
-
-(* Lemma 5.3 Nb originates at n0 *)
-Lemma Nb_origin : Origin (!Nb) n0.
-Proof.
-  (* BOOKMARK *)
-  Admitted.
-
+  Protocol = [NSLInitiator ; NSLResponder].
 
 End NSLSpace.
+
+Export NSLSpace.
